Fixes in concordium extraction (#104)
Fixes in Concordium extraction: derive Reject; more remapping; fix receive wrapper to match the balance update semantics; post-processing of Rust extraction; tests for extracted Escrow

extraction/examples/concordium-extract/escrow-extracted/src/tests.rs
@@ -1,0 +1,172 @@
+// END OF THE GENERATED PART
+
+// The tests are written manually
+#[concordium_cfg_test]
+mod tests {
+    use super::*;
+    use concordium_std::test_infrastructure::*;
+    use std::io::Write;
+
+    // This test writes the init data and reads it back.
+    // Uncomment this test if you want to write the binary
+    // data for making an actual call with concordium-client
+    // NOTE: once uncommented, run is as [cargo test], so
+    // it can write into a file
+   // #[concordium_test]
+    fn test_read_init_data() {
+        let buyer_addr = AccountAddress([0u8; 32]);
+        let setup =
+            ConCert_Execution_Examples_Escrow_Setup::build_setup(PhantomData,
+                                                                 Address::Account(buyer_addr));
+        match std::fs::File::create("escrow_init_data.bin") {
+            Ok(mut f) => {
+                let param_bytes = concert_std::to_bytes(&setup);
+                match f.write_all(&param_bytes) {
+                    Ok(_) =>
+                        match std::fs::read("escrow_init_data.bin") {
+                            Ok(v) => {
+                                let prg = Program::new();
+                                let mut cur = Cursor::new(v);
+                                match <ConCert_Execution_Examples_Escrow_Setup>::concert_deserial(&mut cur, &prg.__alloc) {
+                                    Ok(p) => {
+                                        claim_eq!(p, setup, "Wrong deserial result");
+                                    },
+                                    Err(e) => fail!("{:?}", e)
+                                };
+                            },
+                            Err(e) => fail!("{:?}", e)
+                        },
+                    Err(e) => fail!("Cannot write file: {:?}", e)
+                }
+            },
+            Err(e) => fail!("Cannot create file: {:?}", e)
+        }
+    }
+
+    #[concordium_test]
+    fn test_init() {
+        // buyer_addr should be != seller_addr
+        let buyer_addr = AccountAddress([0u8; 32]);
+        let seller_addr = AccountAddress([1u8; 32]);
+        let amount = 10;
+        let data = Vec::new();
+        let mut st = ContractStateTest::open(data);
+        let mut ctx = InitContextTest::empty();
+        let setup =
+            ConCert_Execution_Examples_Escrow_Setup::build_setup(PhantomData,
+                                                                 Address::Account(buyer_addr));
+        let param_bytes = concert_std::to_bytes(&setup);
+        ctx.set_parameter(&param_bytes);
+        let slot_time = Timestamp::from_timestamp_millis(11);
+        ctx.set_metadata_slot_time(slot_time);
+        ctx.set_init_origin(seller_addr);
+
+
+        // set up the logger so we can intercept and analyze them at the end.
+        let mut logger = LogRecorder::init();
+
+        // call the init function
+        // amount must be even for init to succeed
+        let out = contract_init(&ctx, Amount::from_micro_gtu(amount), &mut logger, &mut st);
+
+        let res = match out {
+            Ok(res) => res,
+            Err(e) => fail!("Contract initialization failed: {:?}", e),
+        };
+        claim_eq!(res, ());
+        let arena = bumpalo::Bump::new();
+        st.seek(SeekFrom::Start(0)).expect("Seek failed");
+        let deserial_state : ConCert_Execution_Examples_Escrow_State = <_>::concert_deserial(&mut st, &arena).expect("Deserialisation failed");
+        let res =  match deserial_state {
+            ConCert_Execution_Examples_Escrow_State::build_state(_, last_action, next_step, seller, buyer, seller_withdrawable, buyer_withdrawable) => {
+                claim_eq!(last_action, slot_time.timestamp_millis(), "Wrong last_action:{:?}",last_action);
+                match next_step {
+                    ConCert_Execution_Examples_Escrow_NextStep::buyer_commit(PhantomData) => (),
+                    _ => fail!("Wrong next_step"),
+                }
+                match seller {
+                    Address::Account(a) => {
+                        claim_eq!(a, seller_addr, "Wrong seller: {:?}", a);
+                    },
+                    _ => fail!("Not an account")
+                };
+                match buyer {
+                    Address::Account(a) => {
+                        claim_eq!(a, buyer_addr, "Wrong buyer: {:?}", a);
+                    },
+                    _ => fail!("Not an account")
+                };
+                claim_eq!(seller_withdrawable, 0, "Wrong seller_withdrawable: {:?}", seller_withdrawable);
+                claim_eq!(buyer_withdrawable, 0, "Wrong buyer_withdrawable: {:?}", buyer_withdrawable);
+            },
+        };
+    }
+
+    #[concordium_test]
+    fn test_receive() {
+        let mut ctx = ReceiveContextTest::empty();
+        let prg = Program::new();
+        let mut data : Vec<u8> = Vec::new();
+        let params = Option::Some(&ConCert_Execution_Examples_Escrow_Msg::commit_money(PhantomData));
+        params.concert_serial(&mut data).expect("Serialisation failed");
+        ctx.set_parameter(&data);
+        let data_st : Vec<u8> = Vec::new();
+        let buyer_addr = AccountAddress([0u8; 32]);
+        let seller_addr = AccountAddress([1u8; 32]);
+        let self_addr = ContractAddress {index: 0, subindex : 0};
+        let amount = 10;
+        let init_balance = 10;
+        let slot_time = Timestamp::from_timestamp_millis(11);
+        ctx.set_metadata_slot_time(slot_time);
+        ctx.set_sender(Address::Account(buyer_addr));
+        ctx.set_self_address(self_addr);
+        ctx.set_self_balance(concordium_std::Amount::from_micro_gtu(init_balance));
+        let mut st = ContractStateTest::open(data_st);
+        let v : ConCert_Execution_Examples_Escrow_State =
+            ConCert_Execution_Examples_Escrow_State::build_state
+            (PhantomData,
+             0,
+             &ConCert_Execution_Examples_Escrow_NextStep::buyer_commit(PhantomData),
+             Address::Account(seller_addr),
+             Address::Account(buyer_addr),
+             0,
+             0);
+        v.concert_serial(&mut st).expect("Serialisation of failed");
+        st.seek(SeekFrom::Start(0)).expect("Seek failed");
+        // set up the logger so we can intercept and analyze them at the end.
+        let mut logger = LogRecorder::init();
+        let res: Result<ActionsTree, _> =
+            contract_receive(&ctx, Amount::from_micro_gtu(amount), &mut logger, &mut st);
+        let actions = match res {
+            Err(e) => fail!("Contract receive failed, but it should not have: {:?}",e),
+            Ok(actions) => actions,
+        };
+        claim_eq!(actions, ActionsTree::Accept, "Contract receive produced incorrect actions.");
+        let arena = bumpalo::Bump::new();
+        st.seek(SeekFrom::Start(0)).expect("Seek failed");
+        let deserial_state : ConCert_Execution_Examples_Escrow_State = <_>::concert_deserial(&mut st, &arena).expect("Deserialisation failed");
+        let res =  match deserial_state {
+            ConCert_Execution_Examples_Escrow_State::build_state(_, last_action, next_step, seller, buyer, seller_withdrawable, buyer_withdrawable) => {
+                claim_eq!(last_action, slot_time.timestamp_millis(), "Wrong last_action:{:?}",last_action);
+                match next_step {
+                    ConCert_Execution_Examples_Escrow_NextStep::buyer_confirm(PhantomData) => (),
+                    _ => fail!("Wrong next_step"),
+                }
+                match seller {
+                    Address::Account(a) => {
+                        claim_eq!(a, seller_addr, "Wrong seller: {:?}", a);
+                    },
+                    _ => fail!("Not an account")
+                };
+                match buyer {
+                    Address::Account(a) => {
+                        claim_eq!(a, buyer_addr, "Wrong buyer: {:?}", a);
+                    },
+                    _ => fail!("Not an account")
+                };
+                claim_eq!(seller_withdrawable, 0, "Wrong seller_withdrawable: {:?}", seller_withdrawable);
+                claim_eq!(buyer_withdrawable, 0, "Wrong buyer_withdrawable: {:?}", buyer_withdrawable);
+            },
+        };
+    }
+}
