extraction/examples/RustEscrow.v
@@ -18,33 +18,21 @@ Definition ESCROW_MODULE : ConcordiumMod _ _ :=
      concmd_receive := @Escrow.receive;
      concmd_extra := []; |}.
 
-Definition null_remap : remapped_inductive :=
-  {| re_ind_name := "()";
-     re_ind_ctors := [];
-     re_ind_match := None |}.
-
-(* Purely remapped so that they are ignored, can be removed when inlining
-   happens on template *)
-Definition extra_remap_inds : list (inductive * remapped_inductive) :=
-  [ (<! Monads.Monad !>, null_remap) ].
-
-Definition extra_remap_consts : list (kername * string) :=
-  [ (<! @RecordSet.SetterFromGetter !>, "") ].
-
 Definition should_inline kn :=
   eq_kername kn <%% @Monads.bind %%>
   || eq_kername kn <%% Monads.Monad_option %%>
   || if String.index 0 "setter_from_getter" (string_of_kername kn) then true else false.
 
-Redirect "examples/rust-extract/Escrow.rs"
+(* NOTE: it is important to declare a priting config, otherwise MetaCoq evaluation tries to normalise a term with an unresolved instance and runs out of memory. *)
+Existing Instance DefaultPrintConfig.RustConfig.
+
+Redirect "examples/concordium-extract/escrow.rs"
 MetaCoq Run (concordium_extraction
                ESCROW_MODULE
                (ConcordiumRemap.build_remaps
                   (ConcordiumRemap.remap_arith
-                     ++ ConcordiumRemap.remap_blockchain_consts
-                     ++ extra_remap_consts)
+                     ++ ConcordiumRemap.remap_blockchain_consts)
                   ConcordiumRemap.remap_inline_bool_ops
                   (ConcordiumRemap.remap_std_types
-                     ++ ConcordiumRemap.remap_blockchain_inductives
-                     ++ extra_remap_inds))
+                     ++ ConcordiumRemap.remap_blockchain_inductives))
                should_inline).
